theories/Monad.v
@@ -1,0 +1,139 @@
+Require Export SepTypes.OrderedType.
+Require Export SepTypes.DownSet.
+
+
+(***
+ *** Monads over Ordered Types
+ ***)
+
+Class MonadOps (M: forall A `{OType A}, Type) : Type :=
+  {
+    returnM : forall {A} `{OType A}, A -> M A;
+    bindM : forall {A B} `{OType A} `{OType B},
+        M A -> (A -> M B) -> M B;
+  }.
+
+Class Monad (M: forall A `{OType A}, Type) `{OTypeF M} `{MonadOps M} : Prop :=
+  {
+    (* Proper-ness requirements *)
+    Proper_returnM {A} `{OType A} :>
+      Proper (oleq ==> oleq) (returnM (M:=M) (A:=A));
+    Proper_bindM {A B} `{OType A} `{OType B} :>
+      Proper (oleq ==> oleq ==> oleq) (bindM (M:=M) (A:=A) (B:=B));
+
+    (* Standard monad laws, which require bind functions to be Proper *)
+    monad_return_bind {A B} `{OType A} `{OType B} a (f : A -> M B) :
+      Proper (oleq ==> oleq) f ->
+      bindM (returnM a) f =o= f a;
+    monad_bind_return {A} `{OType A} (m : M A) :
+      bindM m returnM =o= m;
+    monad_assoc {A B C} `{OType A} `{OType B} `{OType C}
+                m (f: A -> M B) (g: B -> M C) :
+      Proper (oleq ==> oleq) f ->
+      Proper (oleq ==> oleq) g ->
+      bindM (bindM m f) g =o= bindM m (fun x => bindM (f x) g);
+  }.
+
+
+Class MonadStateOps St `{OType St} (M: forall A `{OType A}, Type) : Type :=
+  { getM : M St;
+    putM : St -> M unit;
+  }.
+
+Class MonadState St `{OType St} (M: forall A `{OType A}, Type) `{OTypeF M}
+      `{MonadOps M} `{MonadStateOps St M} : Prop :=
+  {
+    monad_state_monad :> Monad M;
+
+    Proper_putM :> Proper (oleq ==> oleq) putM;
+
+    monad_state_get :
+      forall A `{OType A} (m : M A),
+        bindM getM (fun _ => m) =o= m;
+
+    monad_state_get_put :
+      forall A `{OType A} (f : St -> unit -> M A),
+        bindM getM (fun s => bindM (putM s) (f s))
+        =o= bindM getM (fun s => f s tt);
+
+    monad_state_put_get :
+      forall A `{OType A} s (f : unit -> St -> M A),
+        bindM (putM s) (fun u => bindM getM (f u))
+        =o= bindM (putM s) (fun u => f u s);
+
+    monad_state_put_put :
+      forall A `{OType A} s1 s2 (f : unit -> unit -> M A),
+        bindM (putM s1) (fun u => bindM (putM s2) (f u))
+        =o= bindM (putM s2) (f tt)
+  }.
+
+
+Class MonadFixOps (M: forall A `{OType A}, Type) : Type :=
+  {
+    fixM : forall {A B} `{OType A} `{OType B},
+      ((A -> M B) -> (A -> M B)) -> A -> M B;
+  }.
+
+Class MonadFix (M: forall A `{OType A}, Type)
+      `{OTypeF M} `{MonadFixOps M} : Prop :=
+  {
+    Proper_fixM {A B} `{OType A} `{OType B} :>
+      Proper (oleq ==> oleq) (fixM (M:=M) (A:=A) (B:=B));
+    fixM_correct :
+      forall {A B} `{OType A} `{OType B} (f: (A -> M B) -> (A -> M B)),
+        Proper (oleq ==> oleq) f ->
+        fixM f =o= f (fixM f)
+  }.
+
+Class MonadErrorOps (M: forall A `{OType A}, Type) : Type :=
+  {
+    errorM : forall {A} `{OType A}, M A;
+  }.
+
+Class MonadError (M: forall A `{OType A}, Type)
+      `{OTypeF M} `{MonadOps M} `{MonadErrorOps M} : Prop :=
+  {
+    bindM_errorM :
+      forall {A B} `{OType A} `{OType B} (f: A -> M B),
+        bindM errorM f =o= errorM;
+  }.
+
+
+(***
+ *** The Fixed-Point Monad
+ ***)
+
+Definition FixM A `{OType A} := DownSet A.
+
+Instance OTypeF_FixM : OTypeF FixM := OType_DownSet.
+
+Instance MonadOps_FixM : MonadOps FixM :=
+  { returnM := fun _ _ => downClose;
+    bindM := fun _ _ _ _ => bindDownSet }.
+
+Instance Monad_FixM : Monad FixM.
+Proof.
+  constructor.
+  - apply Proper_downClose.
+  - apply Proper_bindDownSet.
+  - intros; apply DownSet_return_bind; assumption.
+  - intros; apply DownSet_bind_return; assumption.
+  - intros; apply DownSet_assoc.
+Qed.
+
+Instance MonadFixOps_FixM : MonadFixOps FixM :=
+  { fixM := fun _ _ _ _ => fixDownSet }.
+
+Instance MonadFix_FixM : MonadFix FixM.
+Proof.
+  constructor.
+  - intros. admit. (* FIXME: prove this, or fix the property *)
+  - intros. apply fixDownSetUnfold. assumption.
+Admitted.
+
+
+(***
+ *** The Fixed-Point State Monad
+ ***)
+
+(* FIXME... *)
