theories/TraceMonad.v
@@ -1,6 +1,15 @@
-Require Export Coq.Relations.Relations.
-Require Export Coq.Classes.RelationClasses.
-Require Export Coq.Classes.Morphisms.
-Require Export Coq.Setoids.Setoid.
-
 Require Export SepTypes.OrderedType.
+Require Export SepTypes.DownSet.
+Require Export SepTypes.Monad.
+
+Import ListNotations.
+
+
+(***
+ *** The Trace Monad = Final Algebra of Sets of Traces
+ ***)
+
+Definition TraceM St `{OType St} A `{OType A} :
+  St -> DownSet (list St * option A).
+
+FIXME HERE: finish this!
